\documentclass{article}
\usepackage{amsmath}
\usepackage{circuitikz}

\begin{document}
\section*{Coupled Oscilator for 1D System with N Masses}

For this task, a system of N Masses, each with displacement $x_i$, mass of $m$ and spring coeffitients $k_{ij} = \kappa$ for $j = i+1$ and $0$ for others, $k_{ii} = k_{jj} = k$ will be inspected. The equation becomes:

$$| \psi(t) \rangle = \frac{1}{\sqrt{2E}}\begin{pmatrix}
    \sqrt{m}\dot{x}_1(t) \\
    \sqrt{m}\dot{x}_2(t) \\
    \vdots \\
    \sqrt{m}\dot{x}_N(t) \\
    ix_1(t) \\
    ix_2(t) \\
    \vdots \\
    ix_N(t) \\
    i(x_1(t) - x_2(t))\\
    i(x_2(t) - x_3(t))\\
    \vdots \\
    i(x_{N-1}(t) - x_N(t))
\end{pmatrix}$$

Now, in order to find matrix $\textbf{B}$, we have:

$$\sqrt{\textbf{M}}\textbf{B}|1,1\rangle = \sqrt{k}|1\rangle$$
$$\sqrt{\textbf{M}}\textbf{B}|2,2\rangle = \sqrt{k}|2\rangle$$
$$\vdots$$
$$\sqrt{\textbf{M}}\textbf{B}|N,N\rangle = \sqrt{k}|N\rangle$$
$$\sqrt{\textbf{M}}\textbf{B}|1,2\rangle = \sqrt{\kappa}(|1\rangle - |2\rangle)$$
$$\sqrt{\textbf{M}}\textbf{B}|2,3\rangle = \sqrt{\kappa}(|2\rangle - |3\rangle)$$
$$\vdots$$
$$\sqrt{\textbf{M}}\textbf{B}|N-1,N\rangle = \sqrt{\kappa}(|N-1\rangle - |N\rangle)$$

Since $\textbf{M} = \sqrt{m}\textbf{I}$, we have:

$$\textbf{B} = \begin{pmatrix}
    \sqrt{\frac{k}{m}} & 0 & 0 & \dots & 0 & \sqrt{\frac{\kappa}{m}} & 0 & \dots & 0 \\
    0 & \sqrt{\frac{k}{m}} & 0 & \dots & 0 & -\sqrt{\frac{\kappa}{m}} & \sqrt{\frac{\kappa}{m}} & \dots & 0 \\
    0 & 0 & \sqrt{\frac{k}{m}} & \dots & 0 & 0 & -\sqrt{\frac{\kappa}{m}} & \dots & 0 \\
    \vdots & \vdots & \vdots & \ddots & \vdots & \vdots & \vdots & \ddots & \vdots \\
    0 & 0 & 0 & \dots & \sqrt{\frac{k}{m}} & 0 & 0 & \dots & -\sqrt{\frac{\kappa}{m}}
\end{pmatrix}$$

Our hamiltonian will be:

$$\textbf{H} = \begin{pmatrix}
    \textbf{0} & \textbf{B} \\
    \textbf{B}^\dag & \textbf{0}
\end{pmatrix}$$

To find the Pauli string coeffitients, we use the Frobenius norm. The coeffitient for $i$-th Pauli string will be achieved by

$$\alpha_i = \frac{\sqrt{Tr\Bigl[H(\sigma^{(i)}_3\sigma^{(i)}_2\sigma^{(i)}_1\sigma^{(i)}_0)^{\dag}\Bigr]}}{\sqrt{Tr\Bigl[(\sigma^{(i)}_3\sigma^{(i)}_2\sigma^{(i)}_1\sigma^{(i)}_0)(\sigma^{(i)}_3\sigma^{(i)}_2\sigma^{(i)}_1\sigma^{(i)}_0)^{\dag}\Bigr]}}$$

$$\sigma^{(i)} \in \{I, X, Y, Z\}$$

\section*{Hamiltonian of a System of LC Circuits}

Consider an LC circuit with the following components:

\begin{center}
    \begin{circuitikz} \draw
        (0,0) to[L, L=$L_1$] (0,2)
          to[C, C=$C_{11}$] (0,4) -- (1,4)
          (1,4) -- (1,5)
          to[C, C=$C_{22}$] (2.5,5) to[L, L=$L_2$] (4,5) -- (4,4)
        (1,4) -- (1,3) to[C, C=$C_{12}$] (4,3) -- (4,4) -- (5,4)
          (5,4) -- (5,5)
          to[C, C=$C_{33}$] (6.5,5) to[L, L=$L_2$] (8,5) -- (8,4)
        (5,4) -- (5,3) to[C, C=$C_{13}$] (8,3) -- (8,4) -- (9,4)
        (10,4) -- (10.5,4)
          (10.5,4) -- (10.5,5)
          to[C, C=$C_{NN}$] (12,5) to[L, L=$L_N$] (13.5,5) -- (13.5,4)
        (10.5,4) -- (10.5,3) to[C, C=$C_{1N}$] (13.5,3) -- (13.5,4) -- (14,4)
        (14,4) -- (14,0) -- (10,0)
        (9,0) -- (0,0)
        ;
        \node[draw=none] (ellipsis1) at (9.5,4) {$\cdots$};
        \node[draw=none] (ellipsis1) at (9.5,0) {$\cdots$};
    \end{circuitikz}
\end{center}

Let's write the equations of this system based on the charge on each branch. We have

$$L_1\ddot{q_1} = \frac{q_2 - q_1}{C_{12}} + \frac{q_3 - q_1}{C_{13}} + \dots + \frac{q_N - q_1}{C_{1N}} - \frac{q_1}{C_{11}}$$
$$L_2\ddot{q_2} = \frac{q_1 - q_2}{C_{12}} - \frac{q_2}{C_{22}}$$
$$L_3\ddot{q_3} = \frac{q_1 - q_3}{C_{13}} - \frac{q_3}{C_{33}}$$
$$\vdots$$
$$L_N\ddot{q_N} = \frac{q_1 - q_N}{C_{1N}} - \frac{q_N}{C_{NN}}$$

In order to solve this problem, we need to define:

$$m_j = L_j, \quad \kappa_{jk} = \frac{1}{C_{jk}}$$

So, the matrix $B$ need to have:

$$\sqrt{\textbf{M}}\textbf{B}|1,1\rangle = \frac{1}{\sqrt{C_{11}}}|1\rangle$$
$$\sqrt{\textbf{M}}\textbf{B}|2,2\rangle = \frac{1}{\sqrt{C_{22}}}|2\rangle$$
$$\vdots$$
$$\sqrt{\textbf{M}}\textbf{B}|N,N\rangle = \frac{1}{\sqrt{C_{NN}}}|N\rangle$$
$$\sqrt{\textbf{M}}\textbf{B}|1,2\rangle = \frac{1}{\sqrt{C_{12}}}(|1\rangle - |2\rangle)$$
$$\sqrt{\textbf{M}}\textbf{B}|1,3\rangle = \frac{1}{\sqrt{C_{13}}}(|1\rangle - |3\rangle)$$
$$\vdots$$
$$\sqrt{\textbf{M}}\textbf{B}|1,N\rangle = \frac{1}{\sqrt{C_{1N}}}(|1\rangle - |N\rangle)$$

So, the matrix $B$ is:

$$\textbf{B} = \begin{pmatrix}
    \frac{1}{\sqrt{L_1C_{11}}} & 0 & 0 & \dots & 0 & \frac{1}{\sqrt{L_1C_{12}}} & \frac{1}{\sqrt{L_1C_{13}}} & \dots & \frac{1}{\sqrt{L_1C_{1N}}} \\
    0 & \frac{1}{\sqrt{L_2C_{22}}} & 0 & \dots & 0 & -\frac{1}{\sqrt{L_2C_{12}}} & 0 & \dots & 0 \\
    0 & 0 & \frac{1}{\sqrt{L_3C_{33}}} & \dots & 0 & 0 & -\frac{1}{\sqrt{L_3C_{13}}} & \dots & 0 \\
    \vdots & \vdots & \vdots & \ddots & \vdots & \vdots & \vdots & \ddots & \vdots \\
    0 & 0 & 0 & \dots & \frac{1}{\sqrt{L_N C_{NN}}} & 0 & 0 & \dots & -\frac{1}{\sqrt{L_N C_{1N}}}
\end{pmatrix}$$

and the rest can be easily implemented as well.

\end{document}